bernoulli correspondence

Library/Model/Uniform.dfy
@@ -36,12 +36,67 @@ module Uniform {
       Bind(ProbUnif(n / 2), f)
   }
 
+/*   method ProbUnifImperative(n: nat, s: RNG): (t: (nat, RNG)) 
+    ensures t == ProbUnif(n)(s)
+  {
+    var m := 0;
+    var u := 0;
+    while true {
+      m := if Head(s) then 2*m + 1 else 2*m;
+      s := Tail(s);
+      u := 2 * u;
+    }
+  } */
+
+/*   Bind(ProbUnif(n / 2), f)(s)
+  ==
+    var (m, s') := ProbUnif(n / 2)(s);
+    f(m)(s')
+  ==
+    Bind(Deconstruct, (b: bool) => Return(if b then 2*m + 1 else 2*m))(s')
+  ==
+    (b, s'') := Deconstruct(s');
+    Return(if b then 2 * m + 1 else 2 * m)(s'')
+  ==
+    (if b then 2*m + 1 else 2 *m, s'')
+  ==
+    (if Head(s') then 2*m + 1 else 2*m, Tail(s'))
+  == */
+
+
+
   // Definition 49
   function ProbUniform(n: nat): (f: Hurd<nat>)
     requires n > 0
   {
     ProbUnifTerminates(n);
     ProbUntil(ProbUnif(n-1), (x: nat) => x < n)
+  }
+
+  method ProbUniformImperative(n: nat, s: RNG) returns (t: (nat, RNG))
+    requires n > 0
+    ensures t == ProbUniform(n)(s)
+    decreases *
+  {
+    ProbUnifTerminates(n);
+    t := ProbUntilImperative(ProbUnif(n-1), (x: nat) => x < n, s);
+  }
+
+  method ProbUniformImperativeAlternative(n: nat, s: RNG) returns (t: (nat, RNG))
+    requires n > 0
+    ensures t == ProbUniform(n)(s)
+    decreases *
+  {
+    ProbUnifTerminates(n);
+
+    while true
+      decreases *
+    {
+      var (m, s) := ProbUnif(n-1)(s);
+      if m < n {
+        return (m, s);
+      }
+    }
   }
 
   function ProbUniformInterval(a: int, b: int): (f: Hurd<int>)
