Library/Random.dfy
@@ -7,11 +7,15 @@
 
 include "Model/RandomNumberGenerator.dfy"
 include "Model/Model.dfy"
+include "Model/Monad.dfy"
 include "RandomTrait.dfy"
+include "Model/Bernoulli.dfy"
 
 module {:extern "DafnyLibraries"} DafnyLibraries {
   import opened RandomTrait
   import opened RandomNumberGenerator
+  import opened Monad
+  import opened Bernoulli
   import Model
 
   class {:extern} Random extends RandomTrait {
@@ -21,26 +25,34 @@ module {:extern "DafnyLibraries"} DafnyLibraries {
       ensures Model.Coin(old(s)) == (b, s)
 
     // Based on https://arxiv.org/pdf/1304.1916.pdf; unverified.
-    method Uniform(n: nat) returns (u: nat)
-      requires 0 < n
-      ensures Model.Uniform(n)(old(s)) == (u, s)
+    method Uniform(n: nat) returns (m: nat)
+      requires n > 0
+      ensures Model.Uniform(n)(old(s)) == (m, s)
     {
       assume {:axiom} false;
       var v := 1;
-      u := 0;
+      m := 0;
       while true {
         v := 2 * v;
         var b := Coin();
-        u := 2 * u + if b then 1 else 0;
+        m := if b then 2*m + 1 else 2*m;
         if v >= n {
-          if u < n {
+          if m < n {
             return;
           } else {
             v := v - n;
-            u := u - n;
+            m := m - n;
           }
         }
       }
+/*       while true
+        decreases *
+      {
+        var (m, s) := ProbUnif(n-1)(s);
+        if m < n {
+          return (m, s);
+        }
+      } */
     }
     
     method UniformInterval(a: int, b: int) returns (u: int)
@@ -51,36 +63,55 @@ module {:extern "DafnyLibraries"} DafnyLibraries {
       u := a + v;
     }
 
-    // Based on functional version; unverified
     method Bernoulli(p: real) returns (c: bool) 
       decreases *            
       requires 0.0 <= p <= 1.0
       ensures Model.Bernoulli(p)(old(s)) == (c, s) 
     {
-      assume {:axiom} false;
-      var p := p as real;
+      c := true;
+
+      var b := Coin();
+      assert (b, s) == (Head(old(s)), Tail(old(s)));
+      if b {
+        if p <= 0.5 {
+          c := false;
+          assert Model.Bernoulli(p)(old(s)) == (c, s);
+          return;
+        } else {
+          var p := 2.0 * (p as real) - 1.0;
+        }
+      } else {
+        if p <= 0.5 {
+          var p := 2.0 * (p as real);
+        } else {
+          c := true;
+          assert Model.Bernoulli(p)(old(s)) == (c, s);
+          return;
+        }
+      }
+
       while true 
         decreases *
+        invariant (b && p <= 0.5) || (!b && p > 0.5) ==> ProbBernoulliCurried(p, old(s)) == (c, s)
       {
-        var b := Coin();
+        label L:
+        b := Coin();
+        assert (b, s) == (Head(old@L(s)), Tail(old@L(s)));
         if b {
           if p <= 0.5 {
-            return false;
+            c := false;
+            assert Model.Bernoulli(p)(old@L(s)) == (c, s);
+            return;
           } else {
-            calc {
-              1.0 >= (p as real) >= 0.5;
-            ==>
-              2.0 >= 2.0 * (p as real) >= 1.0;
-            ==>
-              1.0 >= 2.0 * (p as real) - 1.0 >= 0.0;
-            }
-            p := 2.0 * (p as real) - 1.0;
+            var p := 2.0 * (p as real) - 1.0;
           }
         } else {
           if p <= 0.5 {
-            p := 2.0 * (p as real);
+            var p := 2.0 * (p as real);
           } else {
-            return true;
+            c := true;
+            assert Model.Bernoulli(p)(old@L(s)) == (c, s);
+            return;
           }
         }
       }
